Regex/NFA/VM/Correctness.lean
@@ -1,8 +1,362 @@
 import Regex.NFA.VM.Basic
 import Regex.NFA.Transition
 
+theorem Array.isEmpty_iff {α} (a : Array α) : a.isEmpty ↔ a = #[] := by
+  have : a.isEmpty ↔ a.data = [] := by
+    simp [Array.isEmpty, Array.size]
+    match a.data with
+    | [] => simp
+    | _ :: _ => simp
+  rw [this]
+  apply Iff.intro
+  . intro h
+    apply Array.ext'
+    simp [h]
+  . intro h
+    simp [h]
+
+theorem Array.mem_back' {a : Array α} (hemp : ¬ a.isEmpty) : a.back' hemp ∈ a := by
+  simp [back', Array.mem_def, Array.getElem_eq_data_get]
+  apply List.get_mem
+
+theorem Array.mem_push (a : Array α) (x y : α) :
+  y ∈ a.push x ↔ y ∈ a ∨ y = x := by
+  unfold Array.push
+  simp [Array.mem_def]
+
+theorem Array.push_pop_eq (a : Array α) (hemp : ¬ a.isEmpty) :
+  a.pop.push (a.back' hemp) = a := by
+  simp at hemp
+  have : 0 < a.size := Nat.pos_of_ne_zero hemp
+  apply Array.ext
+  . simp [Nat.sub_add_cancel this]
+  . simp [Nat.sub_add_cancel this]
+    intro i h _
+    rw [Array.get_push]
+    split
+    case inl h' => rw [Array.getElem_pop]
+    case inr h' =>
+      simp at h'
+      have : i + 1 - 1 ≤ a.size - 1 := Nat.sub_le_sub_right h _
+      simp at this
+      have : i = a.size - 1 := Nat.le_antisymm this h'
+      simp [back', this]
+
+theorem Array.mem_pop (a : Array α) (x : α) (hemp : ¬ a.isEmpty)
+  (mem : x ∈ a) (neq : x ≠ a.back' hemp) : x ∈ a.pop := by
+  rw [←Array.push_pop_eq a hemp] at mem
+  cases (Array.mem_push _ _ _).mp mem with
+  | inl mem => exact mem
+  | inr eq => exact absurd eq neq
+
+theorem Array.mem_pop_or_eq_of_mem (a : Array α) (x : α) (hemp : ¬ a.isEmpty)
+  (mem : x ∈ a) : x ∈ a.pop ∨ x = a.back' hemp := by
+  rw [←Array.push_pop_eq a hemp] at mem
+  exact (Array.mem_push _ _ _).mp mem
+
+theorem Array.mem_of_mem_pop (a : Array α) (x : α) (mem : x ∈ a.pop) :
+  x ∈ a := by
+  cases decEq a.isEmpty true with
+  | isTrue hemp =>
+    have := (Array.isEmpty_iff _).mp hemp
+    subst this
+    simp at mem
+  | isFalse hemp =>
+    rw [←Array.push_pop_eq a hemp]
+    apply (Array.mem_push _ _ _).mpr
+    exact Or.inl mem
+
 namespace NFA.VM
 
-def NodeSet.toSet (ns : NodeSet n) : Set Nat := { i | ∃ h : i < n, ns.get ⟨i, h⟩ }
+theorem mem_εStep_iff_εClosure_sub {nfa : NFA} {S : Set Nat} :
+  (∀ i ∈ S, (_ : i < nfa.nodes.size) → ∀ j ∈ nfa[i].εStep, j ∈ S) ↔
+  ∀ i ∈ S, nfa.εClosure i ⊆ S := by
+  apply Iff.intro
+  . intro assm i mem
+    simp [Set.subset_def]
+    intro k cls
+    induction cls with
+    | base => exact mem
+    | @step i j k step _ ih =>
+      cases Nat.decLt i nfa.nodes.size with
+      | isTrue lt =>
+        simp [getElem?_pos nfa i lt, Option.εStep] at step
+        exact ih (assm i mem lt j step)
+      | isFalse nlt => simp [getElem?_neg nfa i nlt, Option.εStep] at step
+  . intro assm i mem lt j step
+    apply Set.mem_of_mem_of_subset _ (assm i mem)
+    have step' : j ∈ nfa[i]?.εStep := by
+      simp [getElem?_pos nfa i lt, Option.εStep, step]
+    exact NFA.εClosure.step step' .base
+
+theorem εClosureTR_spec {i : Fin nfa.nodes.size} (inBounds : nfa.inBounds) :
+  ∀ j, (εClosureTR nfa inBounds .empty #[i]).get j ↔ j.val ∈ nfa.εClosure i := by
+  let inv (visited : NodeSet nfa.nodes.size) (stack : Array (Fin nfa.nodes.size)) : Prop :=
+    (visited.get i ∨ i ∈ stack) ∧
+    (∀ i j, visited.get i → j.val ∈ nfa[i].εStep → visited.get j ∨ j ∈ stack) ∧
+    (∀ j, (visited.get j ∨ j ∈ stack) → j.val ∈ nfa.εClosure i)
+
+  let rec go (visited : NodeSet nfa.nodes.size) (stack : Array (Fin nfa.nodes.size))
+    (inv₀ : inv visited stack) : inv (εClosureTR nfa inBounds visited stack) #[] := by
+    unfold εClosureTR
+    split
+    case inl hemp =>
+      have : stack = #[] := (Array.isEmpty_iff _).mp hemp
+      exact this ▸ inv₀
+    case inr hemp =>
+      set n := stack.back' hemp with hn
+      set stack' := stack.pop with hs'
+      have : stack.pop.size < stack.size :=
+        Array.lt_size_of_pop_of_not_empty _ hemp
+      cases hvis : visited.get n with
+      | true =>
+        simp [hvis]
+        have inv' : inv visited stack.pop := by
+          apply And.intro
+          . cases inv₀.1 with
+            | inl vis => exact Or.inl vis
+            | inr stk =>
+              cases Nat.decEq i n with
+              | isTrue eq =>
+                have : i = n := Fin.eq_of_val_eq eq
+                exact Or.inl (this ▸ hvis)
+              | isFalse neq =>
+                have : i ≠ n := Fin.ne_of_val_ne neq
+                exact Or.inr (Array.mem_pop _ _ _ stk this)
+          . apply And.intro
+            . intro i j mem step
+              cases inv₀.2.1 i j mem step with
+              | inl vis => exact Or.inl vis
+              | inr stk =>
+                cases decEq j n with
+                | isTrue eq => exact Or.inl (eq ▸ hvis)
+                | isFalse neq => exact Or.inr (Array.mem_pop _ _ _ stk neq)
+            . intro j mem
+              cases mem with
+              | inl vis => exact inv₀.2.2 j (.inl vis)
+              | inr stk =>
+                have : j ∈ stack := Array.mem_of_mem_pop _ _ stk
+                exact inv₀.2.2 j (.inr this)
+        have ih := go visited stack.pop inv'
+        simp at ih
+        exact ih
+      | false =>
+        have : (visited.set n).count_unset < visited.count_unset :=
+          visited.lt_count_unset n.isLt (by simp [hvis])
+        have inBounds' := (inBounds n).right
+        simp [hvis]
+        split
+        next next eqEps =>
+          have h : next < nfa.nodes.size := by
+            rw [hn] at inBounds'
+            simp [Node.εStep, eqEps] at inBounds'
+            exact inBounds'
+
+          set stack'' := stack'.push ⟨next, h⟩ with hs''
+          have inv' : inv (visited.set n) stack'' := by
+            apply And.intro
+            . cases inv₀.1 with
+              | inl vis => simp [NodeSet.get_set_set vis]
+              | inr stk =>
+                cases Array.mem_pop_or_eq_of_mem _ _ hemp stk with
+                | inl stk => exact Or.inr ((Array.mem_push _ _ _).mpr (.inl stk))
+                | inr eq => simp [hn, eq]
+            . apply And.intro
+              . intro i j mem step
+                rw [NodeSet.get_set] at mem
+                split at mem
+                case inl eq =>
+                  simp [eq.symm, eqEps, Node.εStep] at step
+                  exact Or.inr ((Array.mem_push _ _ _).mpr (.inr (Fin.eq_of_val_eq step)))
+                case inr neq =>
+                  cases inv₀.2.1 i j mem step with
+                  | inl vis => simp [NodeSet.get_set_set vis]
+                  | inr stk =>
+                    cases Array.mem_pop_or_eq_of_mem _ _ hemp stk with
+                    | inl stk => exact Or.inr ((Array.mem_push _ _ _).mpr (.inl stk))
+                    | inr eq => simp [hn, eq]
+              . intro j mem
+                cases mem with
+                | inl vis =>
+                  rw [NodeSet.get_set] at vis
+                  split at vis
+                  case inl eq =>
+                    rw [←eq]
+                    exact inv₀.2.2 n (.inr (Array.mem_back' hemp))
+                  case inr _ => exact inv₀.2.2 j (.inl vis)
+                | inr stk =>
+                  cases (Array.mem_push _ _ _).mp stk with
+                  | inl stk =>
+                    have : j ∈ stack := Array.mem_of_mem_pop _ _ stk
+                    exact inv₀.2.2 j (.inr this)
+                  | inr eq =>
+                    simp [eq]
+                    have : n.val ∈ nfa.εClosure i := inv₀.2.2 n (.inr (Array.mem_back' hemp))
+                    exact εClosure_snoc n.isLt this (by simp [Node.εStep, eqEps])
+          have ih := go (visited.set n) stack'' inv'
+          simp at ih
+          exact ih
+        next next₁ next₂ eqSplit =>
+          have h₁ : next₁ < nfa.nodes.size := by
+            rw [hn] at inBounds'
+            simp [Node.εStep, eqSplit] at inBounds'
+            apply Set.mem_of_mem_of_subset (by simp) inBounds'
+          have h₂ : next₂ < nfa.nodes.size := by
+            rw [hn] at inBounds'
+            simp [Node.εStep, eqSplit] at inBounds'
+            apply Set.mem_of_mem_of_subset (by simp) inBounds'
+
+          set stack'' := (stack'.push ⟨next₁, h₁⟩).push ⟨next₂, h₂⟩ with hs''
+          have inv' : inv (visited.set n) stack'' := by
+            apply And.intro
+            . cases inv₀.1 with
+              | inl vis => simp [NodeSet.get_set_set vis]
+              | inr stk =>
+                cases Array.mem_pop_or_eq_of_mem _ _ hemp stk with
+                | inl stk =>
+                  apply Or.inr
+                  apply (Array.mem_push _ _ _).mpr
+                  apply Or.inl
+                  apply (Array.mem_push _ _ _).mpr
+                  exact Or.inl stk
+                | inr eq => simp [hn, eq]
+            . apply And.intro
+              . intro i j mem step
+                rw [NodeSet.get_set] at mem
+                split at mem
+                case inl eq =>
+                  simp [eq.symm, eqSplit, Node.εStep] at step
+                  cases step with
+                  | inl eq₁ =>
+                    apply Or.inr
+                    apply (Array.mem_push _ _ _).mpr
+                    apply Or.inl
+                    apply (Array.mem_push _ _ _).mpr
+                    apply Or.inr
+                    apply Fin.eq_of_val_eq
+                    exact eq₁
+                  | inr eq₂ =>
+                    apply Or.inr
+                    apply (Array.mem_push _ _ _).mpr
+                    apply Or.inr
+                    apply Fin.eq_of_val_eq
+                    exact eq₂
+                case inr neq =>
+                  cases inv₀.2.1 i j mem step with
+                  | inl vis => simp [NodeSet.get_set_set vis]
+                  | inr stk =>
+                    cases Array.mem_pop_or_eq_of_mem _ _ hemp stk with
+                    | inl stk =>
+                      apply Or.inr
+                      apply (Array.mem_push _ _ _).mpr
+                      apply Or.inl
+                      apply (Array.mem_push _ _ _).mpr
+                      exact Or.inl stk
+                    | inr eq => simp [hn, eq]
+              . intro j mem
+                cases mem with
+                | inl vis =>
+                  rw [NodeSet.get_set] at vis
+                  split at vis
+                  case inl eq =>
+                    rw [←eq]
+                    exact inv₀.2.2 n (.inr (Array.mem_back' hemp))
+                  case inr _ => exact inv₀.2.2 j (.inl vis)
+                | inr stk =>
+                  cases (Array.mem_push _ _ _).mp stk with
+                  | inl stk =>
+                    cases (Array.mem_push _ _ _).mp stk with
+                    | inl stk =>
+                      have : j ∈ stack := Array.mem_of_mem_pop _ _ stk
+                      exact inv₀.2.2 j (.inr this)
+                    | inr eq =>
+                      simp [eq]
+                      have : n.val ∈ nfa.εClosure i := inv₀.2.2 n (.inr (Array.mem_back' hemp))
+                      exact εClosure_snoc n.isLt this (by simp [Node.εStep, eqSplit])
+                  | inr eq =>
+                    simp [eq]
+                    have : n.val ∈ nfa.εClosure i := inv₀.2.2 n (.inr (Array.mem_back' hemp))
+                    exact εClosure_snoc n.isLt this (by simp [Node.εStep, eqSplit])
+          have ih := go (visited.set n) stack'' inv'
+          simp at ih
+          exact ih
+        next hne₁ hne₂ =>
+          have inv' : inv (visited.set n) stack.pop := by
+            apply And.intro
+            . cases inv₀.1 with
+              | inl vis =>
+                rw [NodeSet.get_set_set vis]
+                simp
+              | inr stk =>
+                cases Array.mem_pop_or_eq_of_mem _ _ hemp stk with
+                | inl stk => exact Or.inr stk
+                | inr eq => simp [hn, eq]
+            . apply And.intro
+              . intro i j mem step
+                rw [NodeSet.get_set] at mem
+                split at mem
+                case inl eq => simp [eq.symm, Node.εStep] at step
+                case inr neq =>
+                  have := inv₀.2.1 i j mem step
+                  cases this with
+                  | inl vis => simp [NodeSet.get_set_set vis]
+                  | inr stk =>
+                    cases decEq j n with
+                    | isTrue eq => simp [eq]
+                    | isFalse neq =>
+                      apply Or.inr
+                      apply Array.mem_pop _ _ _ stk neq
+              . intro j mem
+                cases mem with
+                | inl vis =>
+                  cases decEq j n with
+                  | isTrue eq =>
+                    simp [eq]
+                    have : n ∈ stack := Array.mem_back' hemp
+                    exact inv₀.2.2 n (.inr this)
+                  | isFalse neq =>
+                    rw [NodeSet.get_set_ne] at vis
+                    . exact inv₀.2.2 j (.inl vis)
+                    . intro h
+                      exact neq (Fin.eq_of_val_eq h).symm
+                | inr stk =>
+                  have : j ∈ stack := Array.mem_of_mem_pop _ _ stk
+                  exact inv₀.2.2 j (.inr this)
+          have ih := go (visited.set n) stack.pop inv'
+          simp at ih
+          exact ih
+
+  have inv₀ : inv .empty #[i] := by
+    simp [inv]
+    exact .base
+  let ⟨h₁, h₂, h₃⟩ := go .empty #[i] inv₀
+  simp at h₁ h₂ h₃
+  intro j
+  apply Iff.intro
+  . exact h₃ j
+  . intro h
+    let S := { j | ∃ j', (εClosureTR nfa inBounds .empty #[i]).get j' ∧ j = j'.val }
+    have mem : i.val ∈ S := by
+      simp
+      exact ⟨i, h₁, rfl⟩
+    have : ∀ j ∈ S, (_ : j < nfa.nodes.size) → ∀ k ∈ nfa[j].εStep, k ∈ S := by
+      intro j mem _ k step
+      simp at mem
+      let ⟨j', h₄, h₅⟩ := mem
+      simp [h₅] at step
+      have klt : k < nfa.nodes.size :=
+        show k ∈ { k | k < nfa.nodes.size} from
+        Set.mem_of_mem_of_subset step (inBounds j').right
+      have := h₂ j' ⟨k, klt⟩ h₄ step
+      simp
+      exact ⟨⟨k, klt⟩, this, rfl⟩
+
+    have := mem_εStep_iff_εClosure_sub.mp this i mem
+    have := Set.mem_of_mem_of_subset h this
+    simp at this
+    let ⟨j', h₄, h₅⟩ := this
+    have : j = j' := Fin.eq_of_val_eq h₅
+    exact this ▸ h₄
+termination_by go _ => (visited.count_unset, stack.size)
 
 end NFA.VM
